test-suite/erasure_live_test.v
@@ -18,13 +18,10 @@ Unset MetaCoq Debug.
 #[local] Existing Instance config.extraction_checker_flags.
 
 Definition test (p : Ast.Env.program) : string :=
-  erase_and_print_template_program default_erasure_config p.
+  erase_and_print_template_program default_erasure_config [] p.
 
 Definition testty (p : Ast.Env.program) : string :=
   typed_erase_and_print_template_program p.
-
-Definition test_fast (p : Ast.Env.program) : string :=
-  erase_fast_and_print_template_program p.
 
 MetaCoq Quote Recursively Definition zero := 0.
 
@@ -53,12 +50,7 @@ Definition singlelim := ((fun (X : Set) (x : X) (e : x = x) =>
 
 Definition erase {A} (a : A) : TemplateMonad unit :=
   aq <- tmQuoteRec a ;;
-  s <- tmEval lazy (erase_and_print_template_program default_erasure_config aq) ;;
-  tmMsg s.
-
-Definition erase_fast {A} (a : A) : TemplateMonad unit :=
-  aq <- tmQuoteRec a ;;
-  s <- tmEval lazy (erase_fast_and_print_template_program aq) ;;
+  s <- tmEval lazy (erase_and_print_template_program default_erasure_config [] aq) ;;
   tmMsg s.
 
 MetaCoq Run (erase 0).
@@ -80,7 +72,6 @@ Definition vplus0123 := (vplus v01 v23).
 Set MetaCoq Timing.
 
 Time MetaCoq Run (tmEval hnf vplus0123 >>= erase).
-Time MetaCoq Run (tmEval hnf vplus0123 >>= erase_fast).
 
 (** Cofix *)
 From Coq Require Import StreamMemo.
@@ -352,7 +343,7 @@ MetaCoq Quote Recursively Definition cbv_provedCopyx :=
 Definition ans_provedCopyx :=
   Eval lazy in (test cbv_provedCopyx).
 MetaCoq Quote Recursively Definition p_provedCopyx := provedCopyx. (* program *)
-Time Definition P_provedCopyx := Eval lazy in (test_fast cbv_provedCopyx).
+Time Definition P_provedCopyx := Eval lazy in (test cbv_provedCopyx).
 (* We don't run this one every time as it is really expensive *)
 (*Time Definition P_provedCopyxvm := Eval vm_compute in (test p_provedCopyx).*)
 
